src/Lean/Elab/PreDefinition/PartialFixpoint/Induction.lean
@@ -66,100 +66,129 @@ private def numberNames (n : Nat) (base : String) : Array Name :=
 def deriveInduction (name : Name) : MetaM Unit :=
   let inductName := name ++ `fixpoint_induct
   realizeConst name inductName do
+  trace[Elab.definition.partialFixpoint] "Called deriveInduction for {inductName}"
   mapError (f := (m!"Cannot derive fixpoint induction principle (please report this issue)\n{indentD ·}")) do
     let some eqnInfo := eqnInfoExt.find? (← getEnv) name |
       throwError "{name} is not defined by partial_fixpoint"
 
-    let infos ← eqnInfo.declNames.mapM getConstInfoDefn
-    -- First open up the fixed parameters everywhere
-    let e' ← eqnInfo.fixedParamPerms.perms[0]!.forallTelescope infos[0]!.type fun xs => do
-      -- Now look at the body of an arbitrary of the functions (they are essentially the same
-      -- up to the final projections)
-      let body ← eqnInfo.fixedParamPerms.perms[0]!.instantiateLambda infos[0]!.value xs
+    if eqnInfo.lattice? then
+      if (eqnInfo.declNames.size != 1) then
+        throwError "Mutual lattice (co)induction is not supported yet"
+      let infos ← eqnInfo.declNames.mapM getConstInfoDefn
+      let e' ← eqnInfo.fixedParamPerms.perms[0]!.forallTelescope infos[0]!.type fun xs => do
+        -- Now look at the body of an arbitrary of the functions (they are essentially the same
+        -- up to the final projections)
+        let body ← eqnInfo.fixedParamPerms.perms[0]!.instantiateLambda infos[0]!.value xs
+        -- We do not strip projections
+        let some fixApp ← whnfUntil body ``gfp_monotone
+          | throwError "Unexpected function body {body}, could not whnfUntil gfp_monotone"
+        let_expr gfp_monotone α instcomplete_lattice F hmono := fixApp
+          | throwError "Unexpected function body {body}, not an application of gfp_coinduction"
+        let e' ← mkAppOptM  ``gfp_coinduction_monotone #[α, instcomplete_lattice, F, hmono]
+        let e' ← mkLambdaFVars (binderInfoForMVars := .default) (usedOnly := true) xs e'
+        let e' ← instantiateMVars e'
+        trace[Elab.definition.partialFixpoint.induction] "complete body of fixpoint induction principle:{indentExpr e'}"
+        pure e'
+      let eTyp ← inferType e'
+      let eTyp ← elimOptParam eTyp
+      -- logInfo m!"eTyp: {eTyp}"
+      let params := (collectLevelParams {} eTyp).params
+      -- Prune unused level parameters, preserving the original order
+      let us := infos[0]!.levelParams.filter (params.contains ·)
 
-      -- The body should now be of the form of the form (fix … ).2.2.1
-      -- We strip the projections (if present)
-      let body' := PProdN.stripProjs body.eta -- TODO: Eta more carefully?
-      let some fixApp ← whnfUntil body' ``fix
-        | throwError "Unexpected function body {body}, could not whnfUntil fix"
-      let_expr fix α instCCPOα F hmono := fixApp
-        | throwError "Unexpected function body {body'}, not an application of fix"
+      addDecl <| Declaration.thmDecl
+        { name := inductName, levelParams := us, type := eTyp, value := e' }
+    else
+      let infos ← eqnInfo.declNames.mapM getConstInfoDefn
+      -- First open up the fixed parameters everywhere
+      let e' ← eqnInfo.fixedParamPerms.perms[0]!.forallTelescope infos[0]!.type fun xs => do
+        -- Now look at the body of an arbitrary of the functions (they are essentially the same
+        -- up to the final projections)
+        let body ← eqnInfo.fixedParamPerms.perms[0]!.instantiateLambda infos[0]!.value xs
 
-      let instCCPOs := CCPOProdProjs infos.size instCCPOα
-      let types ← infos.mapIdxM (eqnInfo.fixedParamPerms.perms[·]!.instantiateForall ·.type xs)
-      let packedType ← PProdN.pack 0 types
-      let motiveTypes ← types.mapM (mkArrow · (.sort 0))
-      let motiveNames := numberNames motiveTypes.size "motive"
-      withLocalDeclsDND (motiveNames.zip motiveTypes) fun motives => do
-        let packedMotive ←
-          withLocalDeclD (← mkFreshUserName `x) packedType fun x => do
-            mkLambdaFVars #[x] <| ← PProdN.pack 0 <|
-              motives.mapIdx fun idx motive =>
-                mkApp motive (PProdN.proj motives.size idx packedType x)
+        -- The body should now be of the form of the form (fix … ).2.2.1
+        -- We strip the projections (if present)
+        let body' := PProdN.stripProjs body.eta -- TODO: Eta more carefully?
+        let some fixApp ← whnfUntil body' ``fix
+          | throwError "Unexpected function body {body}, could not whnfUntil fix"
+        let_expr fix α instCCPOα F hmono := fixApp
+          | throwError "Unexpected function body {body'}, not an application of fix"
 
-        let admTypes ← motives.mapIdxM fun i motive => do
-          mkAppOptM ``admissible #[types[i]!, instCCPOs[i]!, some motive]
-        let admNames := numberNames admTypes.size "adm"
-        withLocalDeclsDND (admNames.zip admTypes) fun adms => do
-          let adms' ← adms.mapIdxM fun i adm => mkAdmProj instCCPOα i adm
-          let packedAdm ← PProdN.genMk (mkAdmAnd α instCCPOα) adms'
-          let hNames := numberNames infos.size "h"
-          let hTypes_hmask : Array (Expr × Array Bool) ← infos.mapIdxM fun i _info => do
-            let approxNames := infos.map fun info =>
-              match info.name with
-                | .str _ n => .mkSimple n
-                | _ => `f
-            withLocalDeclsDND (approxNames.zip types) fun approxs => do
-              let ihTypes := approxs.mapIdx fun j approx => mkApp motives[j]! approx
-              withLocalDeclsDND (ihTypes.map (⟨`ih, ·⟩)) fun ihs => do
-                let f ← PProdN.mk 0 approxs
-                let Ff := F.beta #[f]
-                let Ffi := PProdN.proj motives.size i packedType Ff
-                let t := mkApp motives[i]! Ffi
-                let t ← PProdN.reduceProjs t
-                let mask := approxs.map fun approx => t.containsFVar approx.fvarId!
-                let t ← mkForallFVars (maskArray mask approxs ++ maskArray mask ihs) t
-                pure (t, mask)
-          let (hTypes, masks) := hTypes_hmask.unzip
-          withLocalDeclsDND (hNames.zip hTypes) fun hs => do
-            let packedH ←
-              withLocalDeclD `approx packedType fun approx =>
-                let packedIHType := packedMotive.beta #[approx]
-                withLocalDeclD `ih packedIHType fun ih => do
-                  let approxs := PProdN.projs motives.size packedType approx
-                  let ihs := PProdN.projs motives.size packedIHType ih
-                  let e ← PProdN.mk 0 <| hs.mapIdx fun i h =>
-                    let mask := masks[i]!
-                    mkAppN h (maskArray mask approxs ++ maskArray mask ihs)
-                  mkLambdaFVars #[approx, ih] e
-            let e' ← mkAppOptM ``fix_induct #[α, instCCPOα, F, hmono, packedMotive, packedAdm, packedH]
-            -- Should be the type of e', but with the function definitions folded
-            let packedConclusion ← PProdN.pack 0 <| ←
-              motives.mapIdxM fun i motive => do
-                let f ← mkConstWithLevelParams infos[i]!.name
-                let fEtaExpanded ← lambdaTelescope infos[i]!.value fun ys _ =>
-                  mkLambdaFVars ys (mkAppN f ys)
-                let fInst ← eqnInfo.fixedParamPerms.perms[i]!.instantiateLambda fEtaExpanded xs
-                let fInst := fInst.eta
-                return mkApp motive fInst
-            let e' ← mkExpectedTypeHint e' packedConclusion
-            let e' ← mkLambdaFVars hs e'
-            let e' ← mkLambdaFVars adms e'
-            let e' ← mkLambdaFVars motives e'
-            let e' ← mkLambdaFVars (binderInfoForMVars := .default) (usedOnly := true) xs e'
-            let e' ← instantiateMVars e'
-            trace[Elab.definition.partialFixpoint.induction] "complete body of fixpoint induction principle:{indentExpr e'}"
-            pure e'
+        let instCCPOs := CCPOProdProjs infos.size instCCPOα
+        let types ← infos.mapIdxM (eqnInfo.fixedParamPerms.perms[·]!.instantiateForall ·.type xs)
+        let packedType ← PProdN.pack 0 types
+        let motiveTypes ← types.mapM (mkArrow · (.sort 0))
+        let motiveNames := numberNames motiveTypes.size "motive"
+        withLocalDeclsDND (motiveNames.zip motiveTypes) fun motives => do
+          let packedMotive ←
+            withLocalDeclD (← mkFreshUserName `x) packedType fun x => do
+              mkLambdaFVars #[x] <| ← PProdN.pack 0 <|
+                motives.mapIdx fun idx motive =>
+                  mkApp motive (PProdN.proj motives.size idx packedType x)
 
-    let eTyp ← inferType e'
-    let eTyp ← elimOptParam eTyp
-    -- logInfo m!"eTyp: {eTyp}"
-    let params := (collectLevelParams {} eTyp).params
-    -- Prune unused level parameters, preserving the original order
-    let us := infos[0]!.levelParams.filter (params.contains ·)
+          let admTypes ← motives.mapIdxM fun i motive => do
+            mkAppOptM ``admissible #[types[i]!, instCCPOs[i]!, some motive]
+          let admNames := numberNames admTypes.size "adm"
+          withLocalDeclsDND (admNames.zip admTypes) fun adms => do
+            let adms' ← adms.mapIdxM fun i adm => mkAdmProj instCCPOα i adm
+            let packedAdm ← PProdN.genMk (mkAdmAnd α instCCPOα) adms'
+            let hNames := numberNames infos.size "h"
+            let hTypes_hmask : Array (Expr × Array Bool) ← infos.mapIdxM fun i _info => do
+              let approxNames := infos.map fun info =>
+                match info.name with
+                  | .str _ n => .mkSimple n
+                  | _ => `f
+              withLocalDeclsDND (approxNames.zip types) fun approxs => do
+                let ihTypes := approxs.mapIdx fun j approx => mkApp motives[j]! approx
+                withLocalDeclsDND (ihTypes.map (⟨`ih, ·⟩)) fun ihs => do
+                  let f ← PProdN.mk 0 approxs
+                  let Ff := F.beta #[f]
+                  let Ffi := PProdN.proj motives.size i packedType Ff
+                  let t := mkApp motives[i]! Ffi
+                  let t ← PProdN.reduceProjs t
+                  let mask := approxs.map fun approx => t.containsFVar approx.fvarId!
+                  let t ← mkForallFVars (maskArray mask approxs ++ maskArray mask ihs) t
+                  pure (t, mask)
+            let (hTypes, masks) := hTypes_hmask.unzip
+            withLocalDeclsDND (hNames.zip hTypes) fun hs => do
+              let packedH ←
+                withLocalDeclD `approx packedType fun approx =>
+                  let packedIHType := packedMotive.beta #[approx]
+                  withLocalDeclD `ih packedIHType fun ih => do
+                    let approxs := PProdN.projs motives.size packedType approx
+                    let ihs := PProdN.projs motives.size packedIHType ih
+                    let e ← PProdN.mk 0 <| hs.mapIdx fun i h =>
+                      let mask := masks[i]!
+                      mkAppN h (maskArray mask approxs ++ maskArray mask ihs)
+                    mkLambdaFVars #[approx, ih] e
+              let e' ← mkAppOptM ``fix_induct #[α, instCCPOα, F, hmono, packedMotive, packedAdm, packedH]
+              -- Should be the type of e', but with the function definitions folded
+              let packedConclusion ← PProdN.pack 0 <| ←
+                motives.mapIdxM fun i motive => do
+                  let f ← mkConstWithLevelParams infos[i]!.name
+                  let fEtaExpanded ← lambdaTelescope infos[i]!.value fun ys _ =>
+                    mkLambdaFVars ys (mkAppN f ys)
+                  let fInst ← eqnInfo.fixedParamPerms.perms[i]!.instantiateLambda fEtaExpanded xs
+                  let fInst := fInst.eta
+                  return mkApp motive fInst
+              let e' ← mkExpectedTypeHint e' packedConclusion
+              let e' ← mkLambdaFVars hs e'
+              let e' ← mkLambdaFVars adms e'
+              let e' ← mkLambdaFVars motives e'
+              let e' ← mkLambdaFVars (binderInfoForMVars := .default) (usedOnly := true) xs e'
+              let e' ← instantiateMVars e'
+              trace[Elab.definition.partialFixpoint.induction] "complete body of fixpoint induction principle:{indentExpr e'}"
+              pure e'
 
-    addDecl <| Declaration.thmDecl
-      { name := inductName, levelParams := us, type := eTyp, value := e' }
+      let eTyp ← inferType e'
+      let eTyp ← elimOptParam eTyp
+      -- logInfo m!"eTyp: {eTyp}"
+      let params := (collectLevelParams {} eTyp).params
+      -- Prune unused level parameters, preserving the original order
+      let us := infos[0]!.levelParams.filter (params.contains ·)
+
+      addDecl <| Declaration.thmDecl
+        { name := inductName, levelParams := us, type := eTyp, value := e' }
 
 def isInductName (env : Environment) (name : Name) : Bool := Id.run do
   let .str p s := name | return false
