tests/lean/run/coinductive_predicates.lean
@@ -1,6 +1,7 @@
 open Lean.Order
 
 set_option trace.Elab.definition.partialFixpoint true
+set_option trace.Elab.definition.partialFixpoint.induction true
 
 @[partial_fixpoint_monotone] theorem monotone_exists
     {α} [PartialOrder α] {β} (f : α → β → Prop)
@@ -18,10 +19,15 @@ def infinite_chain {α} (step : α → Option α) (x : α) : Prop :=
   ∃ y, step x = some y ∧ (infinite_chain step y)
   greatest_fixpoint
 
+#check infinite_chain.fixpoint_induct
+
+def infinite_chain_fixpoint {α} (step : α → Option α) (x : α) :
+  infinite_chain step x = ∃ y, step x = some y ∧ infinite_chain step y := by
+    rw [infinite_chain]
+
 theorem infinite_chain.coind {α} (P : α → Prop) (step : α → Option α)
   (h : ∀ (x : α), P x → ∃ y, step x = some y ∧ P y) :
   ∀ x, P x → infinite_chain step x := by
-    unfold infinite_chain
-    unfold gfp_monotone
-    apply (@gfp_coinduction (α → Prop) _)
-    exact h
+    delta infinite_chain
+    apply infinite_chain.fixpoint_induct
+    apply h
